Source/Dafny/Scanner.cs
@@ -211,8 +211,8 @@ public class UTF8Buffer: Buffer {
 public class Scanner {
 	const char EOL = '\n';
 	const int eofSym = 0; /* pdt */
-	const int maxT = 133;
-	const int noSym = 133;
+	const int maxT = 134;
+	const int noSym = 134;
 
 
 	[ContractInvariantMethod]
@@ -517,69 +517,70 @@ public class Scanner {
 			case "multiset": t.kind = 14; break;
 			case "seq": t.kind = 15; break;
 			case "map": t.kind = 16; break;
-			case "assume": t.kind = 28; break;
-			case "calc": t.kind = 29; break;
-			case "case": t.kind = 30; break;
-			case "then": t.kind = 31; break;
-			case "else": t.kind = 32; break;
-			case "decreases": t.kind = 33; break;
-			case "invariant": t.kind = 34; break;
-			case "modifies": t.kind = 35; break;
-			case "reads": t.kind = 36; break;
-			case "requires": t.kind = 37; break;
-			case "include": t.kind = 52; break;
-			case "abstract": t.kind = 53; break;
-			case "module": t.kind = 54; break;
-			case "refines": t.kind = 55; break;
-			case "import": t.kind = 56; break;
-			case "opened": t.kind = 57; break;
-			case "as": t.kind = 59; break;
-			case "default": t.kind = 60; break;
-			case "class": t.kind = 61; break;
-			case "extends": t.kind = 62; break;
-			case "trait": t.kind = 63; break;
-			case "ghost": t.kind = 64; break;
-			case "static": t.kind = 65; break;
-			case "datatype": t.kind = 66; break;
-			case "codatatype": t.kind = 67; break;
-			case "var": t.kind = 68; break;
-			case "newtype": t.kind = 69; break;
-			case "type": t.kind = 70; break;
-			case "iterator": t.kind = 71; break;
-			case "yields": t.kind = 72; break;
-			case "returns": t.kind = 73; break;
-			case "method": t.kind = 74; break;
-			case "lemma": t.kind = 75; break;
-			case "colemma": t.kind = 76; break;
-			case "comethod": t.kind = 77; break;
-			case "constructor": t.kind = 78; break;
-			case "free": t.kind = 79; break;
-			case "ensures": t.kind = 80; break;
-			case "yield": t.kind = 81; break;
-			case "function": t.kind = 82; break;
-			case "predicate": t.kind = 83; break;
-			case "copredicate": t.kind = 84; break;
-			case "label": t.kind = 86; break;
-			case "break": t.kind = 87; break;
-			case "where": t.kind = 88; break;
-			case "return": t.kind = 90; break;
-			case "new": t.kind = 92; break;
-			case "if": t.kind = 93; break;
-			case "while": t.kind = 94; break;
-			case "match": t.kind = 95; break;
-			case "assert": t.kind = 96; break;
-			case "print": t.kind = 97; break;
-			case "forall": t.kind = 98; break;
-			case "parallel": t.kind = 99; break;
-			case "modify": t.kind = 100; break;
-			case "exists": t.kind = 119; break;
-			case "in": t.kind = 121; break;
-			case "false": t.kind = 126; break;
-			case "true": t.kind = 127; break;
-			case "null": t.kind = 128; break;
-			case "this": t.kind = 129; break;
-			case "fresh": t.kind = 130; break;
-			case "old": t.kind = 131; break;
+			case "imap": t.kind = 17; break;
+			case "assume": t.kind = 29; break;
+			case "calc": t.kind = 30; break;
+			case "case": t.kind = 31; break;
+			case "then": t.kind = 32; break;
+			case "else": t.kind = 33; break;
+			case "decreases": t.kind = 34; break;
+			case "invariant": t.kind = 35; break;
+			case "modifies": t.kind = 36; break;
+			case "reads": t.kind = 37; break;
+			case "requires": t.kind = 38; break;
+			case "include": t.kind = 53; break;
+			case "abstract": t.kind = 54; break;
+			case "module": t.kind = 55; break;
+			case "refines": t.kind = 56; break;
+			case "import": t.kind = 57; break;
+			case "opened": t.kind = 58; break;
+			case "as": t.kind = 60; break;
+			case "default": t.kind = 61; break;
+			case "class": t.kind = 62; break;
+			case "extends": t.kind = 63; break;
+			case "trait": t.kind = 64; break;
+			case "ghost": t.kind = 65; break;
+			case "static": t.kind = 66; break;
+			case "datatype": t.kind = 67; break;
+			case "codatatype": t.kind = 68; break;
+			case "var": t.kind = 69; break;
+			case "newtype": t.kind = 70; break;
+			case "type": t.kind = 71; break;
+			case "iterator": t.kind = 72; break;
+			case "yields": t.kind = 73; break;
+			case "returns": t.kind = 74; break;
+			case "method": t.kind = 75; break;
+			case "lemma": t.kind = 76; break;
+			case "colemma": t.kind = 77; break;
+			case "comethod": t.kind = 78; break;
+			case "constructor": t.kind = 79; break;
+			case "free": t.kind = 80; break;
+			case "ensures": t.kind = 81; break;
+			case "yield": t.kind = 82; break;
+			case "function": t.kind = 83; break;
+			case "predicate": t.kind = 84; break;
+			case "copredicate": t.kind = 85; break;
+			case "label": t.kind = 87; break;
+			case "break": t.kind = 88; break;
+			case "where": t.kind = 89; break;
+			case "return": t.kind = 91; break;
+			case "new": t.kind = 93; break;
+			case "if": t.kind = 94; break;
+			case "while": t.kind = 95; break;
+			case "match": t.kind = 96; break;
+			case "assert": t.kind = 97; break;
+			case "print": t.kind = 98; break;
+			case "forall": t.kind = 99; break;
+			case "parallel": t.kind = 100; break;
+			case "modify": t.kind = 101; break;
+			case "exists": t.kind = 120; break;
+			case "in": t.kind = 122; break;
+			case "false": t.kind = 127; break;
+			case "true": t.kind = 128; break;
+			case "null": t.kind = 129; break;
+			case "this": t.kind = 130; break;
+			case "fresh": t.kind = 131; break;
+			case "old": t.kind = 132; break;
 			default: break;
 		}
 	}
@@ -682,7 +683,7 @@ public class Scanner {
 				if (ch >= '0' && ch <= '9' || ch >= 'A' && ch <= 'F' || ch >= 'a' && ch <= 'f') {AddCh(); goto case 15;}
 				else {goto case 0;}
 			case 20:
-				{t.kind = 17; break;}
+				{t.kind = 18; break;}
 			case 21:
 				if (ch <= 9 || ch >= 11 && ch <= 12 || ch >= 14 && ch <= '!' || ch >= '#' && ch <= '[' || ch >= ']' && ch <= 65535) {AddCh(); goto case 21;}
 				else if (ch == '"') {AddCh(); goto case 28;}
@@ -708,37 +709,37 @@ public class Scanner {
 				else if (ch == '"') {AddCh(); goto case 55;}
 				else {goto case 0;}
 			case 28:
-				{t.kind = 18; break;}
+				{t.kind = 19; break;}
 			case 29:
-				{t.kind = 20; break;}
+				{t.kind = 21; break;}
 			case 30:
-				{t.kind = 22; break;}
-			case 31:
 				{t.kind = 23; break;}
+			case 31:
+				{t.kind = 24; break;}
 			case 32:
-				{t.kind = 25; break;}
-			case 33:
 				{t.kind = 26; break;}
-			case 34:
+			case 33:
 				{t.kind = 27; break;}
+			case 34:
+				{t.kind = 28; break;}
 			case 35:
-				{t.kind = 38; break;}
-			case 36:
 				{t.kind = 39; break;}
-			case 37:
+			case 36:
 				{t.kind = 40; break;}
-			case 38:
+			case 37:
 				{t.kind = 41; break;}
-			case 39:
+			case 38:
 				{t.kind = 42; break;}
-			case 40:
+			case 39:
 				{t.kind = 43; break;}
+			case 40:
+				{t.kind = 44; break;}
 			case 41:
-				{t.kind = 47; break;}
-			case 42:
 				{t.kind = 48; break;}
-			case 43:
+			case 42:
 				{t.kind = 49; break;}
+			case 43:
+				{t.kind = 50; break;}
 			case 44:
 				if (ch == 'n') {AddCh(); goto case 45;}
 				else {goto case 0;}
@@ -749,9 +750,9 @@ public class Scanner {
 				{
 					tlen -= apx;
 					SetScannerBehindT();
-					t.kind = 50; break;}
+					t.kind = 51; break;}
 			case 47:
-				{t.kind = 51; break;}
+				{t.kind = 52; break;}
 			case 48:
 				recEnd = pos; recKind = 2;
 				if (ch >= '0' && ch <= '9') {AddCh(); goto case 48;}
@@ -790,9 +791,9 @@ public class Scanner {
 				else if (ch == 'u') {AddCh(); goto case 22;}
 				else {goto case 0;}
 			case 55:
-				recEnd = pos; recKind = 18;
+				recEnd = pos; recKind = 19;
 				if (ch == '"') {AddCh(); goto case 27;}
-				else {t.kind = 18; break;}
+				else {t.kind = 19; break;}
 			case 56:
 				if (ch >= '0' && ch <= '9') {AddCh(); goto case 48;}
 				else {goto case 0;}
@@ -821,9 +822,9 @@ public class Scanner {
 				if (ch == 39 || ch >= '0' && ch <= '9' || ch == '?' || ch >= 'A' && ch <= 'Z' || ch == '_' || ch >= 'a' && ch <= 'z') {AddCh(); goto case 8;}
 				else {t.kind = 1; t.val = new String(tval, 0, tlen); CheckLiteral(); return t;}
 			case 62:
-				recEnd = pos; recKind = 17;
+				recEnd = pos; recKind = 18;
 				if (ch == 39 || ch >= '0' && ch <= '9' || ch == '?' || ch >= 'A' && ch <= 'Z' || ch == '_' || ch >= 'a' && ch <= 'z') {AddCh(); goto case 8;}
-				else {t.kind = 17; break;}
+				else {t.kind = 18; break;}
 			case 63:
 				recEnd = pos; recKind = 1;
 				if (ch == 39 || ch >= '0' && ch <= '9' || ch == '?' || ch >= 'A' && ch <= 'Z' || ch == '_' || ch >= 'a' && ch <= 'x' || ch == 'z') {AddCh(); goto case 5;}
@@ -840,104 +841,104 @@ public class Scanner {
 				else if (ch >= '0' && ch <= '9') {AddCh(); goto case 65;}
 				else {t.kind = 5; break;}
 			case 66:
-				{t.kind = 85; break;}
+				{t.kind = 86; break;}
 			case 67:
-				{t.kind = 89; break;}
+				{t.kind = 90; break;}
 			case 68:
-				{t.kind = 91; break;}
+				{t.kind = 92; break;}
 			case 69:
-				{t.kind = 101; break;}
+				{t.kind = 102; break;}
 			case 70:
-				{t.kind = 103; break;}
-			case 71:
 				{t.kind = 104; break;}
-			case 72:
+			case 71:
 				{t.kind = 105; break;}
-			case 73:
+			case 72:
 				{t.kind = 106; break;}
-			case 74:
+			case 73:
 				{t.kind = 107; break;}
-			case 75:
+			case 74:
 				{t.kind = 108; break;}
-			case 76:
+			case 75:
 				{t.kind = 109; break;}
+			case 76:
+				{t.kind = 110; break;}
 			case 77:
-				{t.kind = 111; break;}
+				{t.kind = 112; break;}
 			case 78:
 				if (ch == '&') {AddCh(); goto case 79;}
 				else {goto case 0;}
 			case 79:
-				{t.kind = 112; break;}
-			case 80:
 				{t.kind = 113; break;}
-			case 81:
+			case 80:
 				{t.kind = 114; break;}
-			case 82:
+			case 81:
 				{t.kind = 115; break;}
+			case 82:
+				{t.kind = 116; break;}
 			case 83:
-				{t.kind = 117; break;}
-			case 84:
 				{t.kind = 118; break;}
+			case 84:
+				{t.kind = 119; break;}
 			case 85:
-				{t.kind = 120; break;}
+				{t.kind = 121; break;}
 			case 86:
-				{t.kind = 122; break;}
+				{t.kind = 123; break;}
 			case 87:
-				{t.kind = 124; break;}
-			case 88:
 				{t.kind = 125; break;}
+			case 88:
+				{t.kind = 126; break;}
 			case 89:
-				recEnd = pos; recKind = 19;
+				recEnd = pos; recKind = 20;
 				if (ch == ':') {AddCh(); goto case 30;}
 				else if (ch == '=') {AddCh(); goto case 67;}
 				else if (ch == '|') {AddCh(); goto case 68;}
-				else {t.kind = 19; break;}
+				else {t.kind = 20; break;}
 			case 90:
-				recEnd = pos; recKind = 21;
+				recEnd = pos; recKind = 22;
 				if (ch == '|') {AddCh(); goto case 81;}
-				else {t.kind = 21; break;}
+				else {t.kind = 22; break;}
 			case 91:
-				recEnd = pos; recKind = 24;
+				recEnd = pos; recKind = 25;
 				if (ch == '.') {AddCh(); goto case 97;}
-				else {t.kind = 24; break;}
+				else {t.kind = 25; break;}
 			case 92:
-				recEnd = pos; recKind = 58;
+				recEnd = pos; recKind = 59;
 				if (ch == '>') {AddCh(); goto case 33;}
 				else if (ch == '=') {AddCh(); goto case 98;}
-				else {t.kind = 58; break;}
+				else {t.kind = 59; break;}
 			case 93:
-				recEnd = pos; recKind = 123;
+				recEnd = pos; recKind = 124;
 				if (ch == '>') {AddCh(); goto case 34;}
-				else {t.kind = 123; break;}
+				else {t.kind = 124; break;}
 			case 94:
-				recEnd = pos; recKind = 44;
-				if (ch == '=') {AddCh(); goto case 99;}
-				else {t.kind = 44; break;}
-			case 95:
 				recEnd = pos; recKind = 45;
-				if (ch == '=') {AddCh(); goto case 70;}
+				if (ch == '=') {AddCh(); goto case 99;}
 				else {t.kind = 45; break;}
+			case 95:
+				recEnd = pos; recKind = 46;
+				if (ch == '=') {AddCh(); goto case 70;}
+				else {t.kind = 46; break;}
 			case 96:
-				recEnd = pos; recKind = 116;
+				recEnd = pos; recKind = 117;
 				if (ch == '=') {AddCh(); goto case 41;}
 				else if (ch == 'i') {AddCh(); goto case 44;}
-				else {t.kind = 116; break;}
+				else {t.kind = 117; break;}
 			case 97:
-				recEnd = pos; recKind = 132;
+				recEnd = pos; recKind = 133;
 				if (ch == '.') {AddCh(); goto case 47;}
-				else {t.kind = 132; break;}
+				else {t.kind = 133; break;}
 			case 98:
-				recEnd = pos; recKind = 46;
+				recEnd = pos; recKind = 47;
 				if (ch == '>') {AddCh(); goto case 75;}
-				else {t.kind = 46; break;}
+				else {t.kind = 47; break;}
 			case 99:
-				recEnd = pos; recKind = 102;
+				recEnd = pos; recKind = 103;
 				if (ch == '=') {AddCh(); goto case 100;}
-				else {t.kind = 102; break;}
+				else {t.kind = 103; break;}
 			case 100:
-				recEnd = pos; recKind = 110;
+				recEnd = pos; recKind = 111;
 				if (ch == '>') {AddCh(); goto case 73;}
-				else {t.kind = 110; break;}
+				else {t.kind = 111; break;}
 
 		}
 		t.val = new String(tval, 0, tlen);
